src/FcEtt/fix_typing.v
@@ -156,7 +156,7 @@ Proof.
     { eapply E_App_intro; simpl; eauto.
       { eapply E_IApp_intro with (a := (a_Var_f X)); simpl; eauto.
 
-        pose (K := @E_Fam _ Fix  (erase_tm FixTy Nom) Nom (erase_tm FixDef Nom) H1).
+        pose (K := @E_Fam _ Fix Nom (erase_tm FixTy Nom) (erase_tm FixDef Nom) H1).
         unfold toplevel, erase_sig in K.
         apply binds_map with 
           (f:=fun s : sig_sort => erase_csort s Nom) in H.
